examples/stateful_bignum/multiplication_st.fst
@@ -38,8 +38,10 @@ let rec bitweight_lemma_0 t i j =
 val auxiliary_lemma_1: t:template{ forall (n:nat). t n = t 0 } -> a:nat -> b:nat -> 
 		       Lemma (ensures ( pow2 (bitweight t (a+b)) = pow2 (bitweight t a) * pow2 (bitweight t b)))
 let auxiliary_lemma_1 t a b =
-  bitweight_lemma_0 t a b;
-  pow2_exp_lemma (bitweight t a) (bitweight t b)
+  erase (
+    bitweight_lemma_0 t a b;
+    pow2_exp_lemma (bitweight t a) (bitweight t b)
+  )
 
 (* Lemma : first half of the helper for the multiplication_step_lemma *)
 val multiplication_step_lemma_p1:
@@ -65,28 +67,30 @@ val multiplication_step_lemma_p1:
 	     ))
 
 let multiplication_step_lemma_p1 h0 h1 a b c idx len =
-  auxiliary_lemma_0 len idx 1;
-  cut (eval h1 c (len+idx-1) = eval h0 a (len+idx-1) + (pow2 (bitweight (Bigint63.t a) idx)) * eval h0 b (len-1) /\ True);
-  cut (getValue h1 c (len+idx-1) = getValue h0 a (len+idx-1) + getValue h0 b (len-1) /\ True);
-  cut (eval h1 c (len+idx) = eval h1 c (len+idx-1) + pow2 (bitweight (Bigint63.t a) (len+idx-1)) * (getValue h1 c (len+idx-1)) /\ True );
-  cut (eval h1 c (len+idx) = 
-	 eval h0 a (len+idx-1) + (pow2 (bitweight (Bigint63.t a) idx)) * eval h0 b (len-1)
-	 +
-	   pow2 (bitweight (Bigint63.t a) (len-1+idx)) * (getValue h0 a (len+idx-1) + getValue h0 b (len-1)) /\ True);
-  distributivity_add_right (pow2 (bitweight (Bigint63.t a) (len-1+idx))) (getValue h0 a (len+idx-1)) (getValue h0 b (len-1));
-  cut (True /\ eval h1 c (len+idx) = 
-	 eval h0 a (len+idx-1) + (pow2 (bitweight (Bigint63.t a) idx)) * eval h0 b (len-1)
-	 +
-	   pow2 (bitweight (Bigint63.t a) (len-1+idx)) * getValue h0 a (len+idx-1) + 
-           pow2 (bitweight (Bigint63.t a) (len-1+idx)) * getValue h0 b (len-1));
-  cut (True /\ eval h1 c (len+idx) = 
-	 pow2 (bitweight (Bigint63.t a) (len-1+idx)) * getValue h0 a (len+idx-1) + eval h0 a (len+idx-1) + 
-           pow2 (bitweight (Bigint63.t a) idx) * eval h0 b (len-1)  +	        
-           pow2 (bitweight (Bigint63.t a) (len-1+idx)) * getValue h0 b (len-1));
-  cut (True /\ eval h0 a (len+idx) = pow2 (bitweight (Bigint63.t a) (len-1+idx)) * getValue h0 a (len+idx-1) + eval h0 a (len+idx-1));
-  cut (True /\ eval h1 c (len+idx) = eval h0 a (len+idx) +  
-				       pow2 (bitweight (Bigint63.t a) idx) * eval h0 b (len-1)  +	        
-				       pow2 (bitweight (Bigint63.t a) (len-1+idx)) * getValue h0 b (len-1))
+  erase (
+    auxiliary_lemma_0 len idx 1;
+    cut (eval h1 c (len+idx-1) = eval h0 a (len+idx-1) + (pow2 (bitweight (Bigint63.t a) idx)) * eval h0 b (len-1) /\ True);
+    cut (getValue h1 c (len+idx-1) = getValue h0 a (len+idx-1) + getValue h0 b (len-1) /\ True);
+    cut (eval h1 c (len+idx) = eval h1 c (len+idx-1) + pow2 (bitweight (Bigint63.t a) (len+idx-1)) * (getValue h1 c (len+idx-1)) /\ True );
+    cut (eval h1 c (len+idx) = 
+	eval h0 a (len+idx-1) + (pow2 (bitweight (Bigint63.t a) idx)) * eval h0 b (len-1)
+	+
+	  pow2 (bitweight (Bigint63.t a) (len-1+idx)) * (getValue h0 a (len+idx-1) + getValue h0 b (len-1)) /\ True);
+    distributivity_add_right (pow2 (bitweight (Bigint63.t a) (len-1+idx))) (getValue h0 a (len+idx-1)) (getValue h0 b (len-1));
+    cut (True /\ eval h1 c (len+idx) = 
+	eval h0 a (len+idx-1) + (pow2 (bitweight (Bigint63.t a) idx)) * eval h0 b (len-1)
+	+
+	  pow2 (bitweight (Bigint63.t a) (len-1+idx)) * getValue h0 a (len+idx-1) + 
+          pow2 (bitweight (Bigint63.t a) (len-1+idx)) * getValue h0 b (len-1));
+    cut (True /\ eval h1 c (len+idx) = 
+	pow2 (bitweight (Bigint63.t a) (len-1+idx)) * getValue h0 a (len+idx-1) + eval h0 a (len+idx-1) + 
+          pow2 (bitweight (Bigint63.t a) idx) * eval h0 b (len-1)  +	        
+          pow2 (bitweight (Bigint63.t a) (len-1+idx)) * getValue h0 b (len-1));
+    cut (True /\ eval h0 a (len+idx) = pow2 (bitweight (Bigint63.t a) (len-1+idx)) * getValue h0 a (len+idx-1) + eval h0 a (len+idx-1));
+    cut (True /\ eval h1 c (len+idx) = eval h0 a (len+idx) +  
+	pow2 (bitweight (Bigint63.t a) idx) * eval h0 b (len-1)  +	        
+	pow2 (bitweight (Bigint63.t a) (len-1+idx)) * getValue h0 b (len-1))
+  )
 
 (* Lemma : second half of the helper for the multiplciation_step_lemma *)
 val multiplication_step_lemma_p2:
@@ -109,19 +113,20 @@ val multiplication_step_lemma_p2:
 	     ))
 
 let multiplication_step_lemma_p2 h0 h1 a b c idx len =
-  auxiliary_lemma_0 len idx 1;
-  auxiliary_lemma_1 (Bigint63.t a) idx (len-1);
-  cut (True /\ pow2 (bitweight (Bigint63.t a) (len-1+idx)) = pow2 (bitweight (Bigint63.t a) idx) * pow2 (bitweight (Bigint63.t a) (len-1)) );
-  paren_mul_left (pow2 (bitweight (Bigint63.t a) idx)) (pow2 (bitweight (Bigint63.t a) (len-1))) (getValue h0 b (len-1));
-  cut (eval h1 c (len+idx) = eval h0 a (len+idx) +  
-                          pow2 (bitweight (Bigint63.t a) idx) * eval h0 b (len-1)  +	        
-			  pow2 (bitweight (Bigint63.t a) idx) * pow2 (bitweight (Bigint63.t a) (len-1)) * getValue h0 b (len-1) /\ True);
-  distributivity_add_right (pow2 (bitweight (Bigint63.t a) idx)) (eval h0 b (len-1)) (pow2 (bitweight (Bigint63.t a) (len-1)) * (getValue h0 b (len-1)));     
-  cut (True /\ eval h0 b len = eval h0 b (len-1) + (pow2 (bitweight (Bigint63.t a) (len-1))) * (getValue h0 b (len-1)) );  
-  cut (True /\ pow2 (bitweight (Bigint63.t a) (len-1+idx)) * getValue h0 b (len-1) =
-         pow2 (bitweight (Bigint63.t a) idx) * pow2 (bitweight (Bigint63.t a) (len-1)) * getValue h0 b (len-1) );
-  cut ( True /\ eval h1 c (len+idx) = eval h0 a (len+idx) + pow2 (bitweight (Bigint63.t a) idx) * eval h0 b len) 
-
+  erase (
+    auxiliary_lemma_0 len idx 1;
+    auxiliary_lemma_1 (Bigint63.t a) idx (len-1);
+    cut (True /\ pow2 (bitweight (Bigint63.t a) (len-1+idx)) = pow2 (bitweight (Bigint63.t a) idx) * pow2 (bitweight (Bigint63.t a) (len-1)) );
+    paren_mul_left (pow2 (bitweight (Bigint63.t a) idx)) (pow2 (bitweight (Bigint63.t a) (len-1))) (getValue h0 b (len-1));
+    cut (eval h1 c (len+idx) = eval h0 a (len+idx) +  
+        pow2 (bitweight (Bigint63.t a) idx) * eval h0 b (len-1)  +	        
+	pow2 (bitweight (Bigint63.t a) idx) * pow2 (bitweight (Bigint63.t a) (len-1)) * getValue h0 b (len-1) /\ True);
+    distributivity_add_right (pow2 (bitweight (Bigint63.t a) idx)) (eval h0 b (len-1)) (pow2 (bitweight (Bigint63.t a) (len-1)) * (getValue h0 b (len-1)));     
+    cut (True /\ eval h0 b len = eval h0 b (len-1) + (pow2 (bitweight (Bigint63.t a) (len-1))) * (getValue h0 b (len-1)) );  
+    cut (True /\ pow2 (bitweight (Bigint63.t a) (len-1+idx)) * getValue h0 b (len-1) =
+        pow2 (bitweight (Bigint63.t a) idx) * pow2 (bitweight (Bigint63.t a) (len-1)) * getValue h0 b (len-1) );
+    cut ( True /\ eval h1 c (len+idx) = eval h0 a (len+idx) + pow2 (bitweight (Bigint63.t a) idx) * eval h0 b len) 
+  )
 
 (* Lemma : changes the result of the addition function into the equivalent relation between 
   evaluated bigints *)
@@ -145,15 +150,16 @@ val multiplication_step_lemma:
 	     ))
 
 let rec multiplication_step_lemma h0 h1 a b c idx len =
-  match len with
-  | 0 ->
-     admit () //eval_eq_lemma h0 h1 a c idx
-  | _ ->
-     auxiliary_lemma_0 len idx 1;
-     multiplication_step_lemma h0 h1 a b c idx (len-1);
-     multiplication_step_lemma_p1 h0 h1 a b c idx len;
-     multiplication_step_lemma_p2 h0 h1 a b c idx len
-
+  erase (
+    match len with
+    | 0 ->
+       admit () //eval_eq_lemma h0 h1 a c idx
+    | _ ->
+       auxiliary_lemma_0 len idx 1;
+      multiplication_step_lemma h0 h1 a b c idx (len-1);
+      multiplication_step_lemma_p1 h0 h1 a b c idx len;
+      multiplication_step_lemma_p2 h0 h1 a b c idx len
+  )
 #reset-options
 
 (* Helper lemmas that avoid super long computation or intensive use of "cuts" *)
@@ -271,17 +277,19 @@ val auxiliary_lemma_2:
 	    /\ (maxValue h1 b <= pow2 ((wordSize b - log (getLength h0 a) - 2 ) / 2))))
 
 let auxiliary_lemma_2 h0 h1 h2 a b ctr c =
-  cut ( maxValue h0 a <= pow2 (maxSize h0 a) /\ True );
-  if (((wordSize a - log (getLength h0 a) - 2) / 2) > (maxSize h0 a)) then
-    pow2_increases_lemma ((wordSize a - log (getLength h0 a) - 2) / 2) (maxSize h0 a);
-  if (((wordSize b - log (getLength h1 b) - 2) / 2) > (maxSize h1 b)) then
-    pow2_increases_lemma ((wordSize b - log (getLength h1 b) - 2) / 2) (maxSize h1 b);
-  cut (pow2 (maxSize h0 a) <= pow2 ((wordSize a - log (getLength h0 a) - 2) / 2) /\ True );
-  cut (maxValue h0 a <= pow2 (maxSize h0 a) /\ True );
-  cut (maxValue h0 a <= pow2 ((wordSize a - log (getLength h0 a) - 2) / 2 ) /\ True );
-  cut (pow2 (maxSize h1 b) <= pow2 ((wordSize b - log (getLength h1 b) - 2) / 2) /\ True );
-  cut (maxValue h1 b <= pow2 (maxSize h1 b) /\ True );
-  cut (maxValue h1 b <= pow2 ((wordSize b - log (getLength h1 b) - 2) / 2 ) /\ True )
+  erase (
+    cut ( maxValue h0 a <= pow2 (maxSize h0 a) /\ True );
+    if (((wordSize a - log (getLength h0 a) - 2) / 2) > (maxSize h0 a)) then
+      pow2_increases_lemma ((wordSize a - log (getLength h0 a) - 2) / 2) (maxSize h0 a);
+    if (((wordSize b - log (getLength h1 b) - 2) / 2) > (maxSize h1 b)) then
+      pow2_increases_lemma ((wordSize b - log (getLength h1 b) - 2) / 2) (maxSize h1 b);
+    cut (pow2 (maxSize h0 a) <= pow2 ((wordSize a - log (getLength h0 a) - 2) / 2) /\ True );
+    cut (maxValue h0 a <= pow2 (maxSize h0 a) /\ True );
+    cut (maxValue h0 a <= pow2 ((wordSize a - log (getLength h0 a) - 2) / 2 ) /\ True );
+    cut (pow2 (maxSize h1 b) <= pow2 ((wordSize b - log (getLength h1 b) - 2) / 2) /\ True );
+    cut (maxValue h1 b <= pow2 (maxSize h1 b) /\ True );
+    cut (maxValue h1 b <= pow2 ((wordSize b - log (getLength h1 b) - 2) / 2 ) /\ True )
+  )
   
 #reset-options
 
@@ -400,22 +408,23 @@ val multiplication_step_resize :
      ))
 
 let multiplication_step_resize a b ctr c =
-  let h0 = ST.get() in
-  let s = (wordSize a - log (getLength h0 a) - 2) in
-  auxiliary_lemma_3 h0 h0 h0 a b ctr c;
-  cut ( maxValue h0 a * maxValue h0 b <= pow2 s /\ True);
-  helper_lemma_4 (maxValue h0 a) (maxValue h0 b);
-  mul_incr_lemma ctr (maxValue h0 a * maxValue h0 b) (pow2 s);
-  cut (maxValue h0 c <= ctr * pow2 s /\ True);
-  size_lemma_2 h0 c ctr s;
-  cut ( forall (i:nat). i < getLength h0 c ==> Bitsize (getValue h0 c i) (sizeOf ctr + s) );
-  if ctr < getLength h0 a then log_incr_lemma ctr (getLength h0 a);
-  cut (sizeOf ctr + s <= wordSize a - 2 /\ True );
-  if (sizeOf ctr + s < wordSize a - 2) then pow2_increases_lemma (wordSize a - 2) (sizeOf ctr + s);
-  cut ( forall (i:nat). i < getLength h0 c ==> Bitsize (getValue h0 c i) (wordSize a - 2) );
-  let new_size = wordSize a - 2 in
-  multiplication_step_resize_iterate c new_size (getLength h0 c)
-
+  erase (
+    let h0 = ST.get() in
+    let s = (wordSize a - log (getLength h0 a) - 2) in
+    auxiliary_lemma_3 h0 h0 h0 a b ctr c;
+    cut ( maxValue h0 a * maxValue h0 b <= pow2 s /\ True);
+    helper_lemma_4 (maxValue h0 a) (maxValue h0 b);
+    mul_incr_lemma ctr (maxValue h0 a * maxValue h0 b) (pow2 s);
+    cut (maxValue h0 c <= ctr * pow2 s /\ True);
+    size_lemma_2 h0 c ctr s;
+    cut ( forall (i:nat). i < getLength h0 c ==> Bitsize (getValue h0 c i) (sizeOf ctr + s) );
+    if ctr < getLength h0 a then log_incr_lemma ctr (getLength h0 a);
+    cut (sizeOf ctr + s <= wordSize a - 2 /\ True );
+    if (sizeOf ctr + s < wordSize a - 2) then pow2_increases_lemma (wordSize a - 2) (sizeOf ctr + s);
+    cut ( forall (i:nat). i < getLength h0 c ==> Bitsize (getValue h0 c i) (wordSize a - 2) );
+    let new_size = wordSize a - 2 in
+    multiplication_step_resize_iterate c new_size (getLength h0 c)
+  )
 
 #reset-options
 
@@ -449,16 +458,17 @@ val auxiliary_lemma_5:
     (ensures ( (eval h1 b len2 = eval h0 a len2 + c)))
 
 let rec auxiliary_lemma_5 h0 h1 a b c len len2 =
-  match len2 - len with
-  | 0 -> ()
-  | _ ->
-     let t = Bigint63.t a in
-     auxiliary_lemma_5 h0 h1 a b c len (len2-1);
-     cut (True /\ eval h1 b (len2-1) = eval h0 a (len2-1) + c);
-     cut (True /\ eval h1 b len2 = eval h1 b (len2-1) + (pow2 (bitweight t (len2-1))) * getValue h1 b (len2-1));
-     cut (True /\ eval h1 b len2 = eval h0 a (len2-1) + c + (pow2 (bitweight t (len2-1))) * getValue h0 a (len2-1));
-     cut (True /\ eval h1 b len2 = eval h0 a len2 + c)
-
+  erase (
+    match len2 - len with
+    | 0 -> ()
+    | _ ->
+       let t = Bigint63.t a in
+       auxiliary_lemma_5 h0 h1 a b c len (len2-1);
+       cut (True /\ eval h1 b (len2-1) = eval h0 a (len2-1) + c);
+       cut (True /\ eval h1 b len2 = eval h1 b (len2-1) + (pow2 (bitweight t (len2-1))) * getValue h1 b (len2-1));
+       cut (True /\ eval h1 b len2 = eval h0 a (len2-1) + c + (pow2 (bitweight t (len2-1))) * getValue h0 a (len2-1));
+       cut (True /\ eval h1 b len2 = eval h0 a len2 + c)
+  )
 
 (* Same as auxiliary_lemma_4, TODO : remove *)
 val auxiliary_lemma_6 : ha:heap -> hb:heap -> a:bigint{ inHeap ha a } -> b:bigint{ inHeap hb b } ->
@@ -671,11 +681,12 @@ let multiplication_step a b ctr c tmp =
   multiplication_step_resize a b (ctr+1) c;
   let h2 = 
     erase (ST.get()) in
-  eval_eq_lemma h1 h2 c c (getLength h1 c);
-  swap_mul (eval h0 a (getLength h0 a) * getValue h0 b ctr) (pow2 (bitweight (Bigint63.t a) ctr));
-  paren_mul_left (eval h0 a (getLength h0 a)) (getValue h0 b ctr) (pow2 (bitweight (Bigint63.t a) ctr));
-  ()
-
+  erase (
+    eval_eq_lemma h1 h2 c c (getLength h1 c);
+    swap_mul (eval h0 a (getLength h0 a) * getValue h0 b ctr) (pow2 (bitweight (Bigint63.t a) ctr));
+    paren_mul_left (eval h0 a (getLength h0 a)) (getValue h0 b ctr) (pow2 (bitweight (Bigint63.t a) ctr));
+    ()
+  )
 
 (* Lemma : factorizes "eval" equation *)
 val multiplication_step_lemma_2:
@@ -694,17 +705,18 @@ val multiplication_step_lemma_2:
     (ensures ( eval h1 c (getLength h1 c) = eval h0 a (getLength h0 a) * eval h0 b (getLength h0 a - ctr + 1)))
 
 let multiplication_step_lemma_2 h0 h1 a b ctr c =
-  let t = Bigint63.t a in
-  let len_a = getLength h0 a in
-  paren_mul_left (eval h0 a len_a) (getValue h0 b (len_a - ctr)) (pow2 (bitweight t (len_a - ctr)));
-  cut (True /\ eval h1 c (getLength h1 c) = eval h0 a len_a * getValue h0 b (len_a - ctr) * pow2 (bitweight t (len_a - ctr)) + eval h0 a len_a * eval h0 b (len_a - ctr) );
-  swap_mul (getValue h0 b (len_a - ctr)) (pow2 (bitweight t (len_a - ctr)));
-  cut (True /\ eval h1 c (getLength h1 c) = eval h0 a len_a * pow2 (bitweight t (len_a - ctr)) * getValue h0 b (len_a - ctr) + eval h0 a len_a * eval h0 b (len_a - ctr) ) ;
+  erase (
+    let t = Bigint63.t a in
+    let len_a = getLength h0 a in
+    paren_mul_left (eval h0 a len_a) (getValue h0 b (len_a - ctr)) (pow2 (bitweight t (len_a - ctr)));
+    cut (True /\ eval h1 c (getLength h1 c) = eval h0 a len_a * getValue h0 b (len_a - ctr) * pow2 (bitweight t (len_a - ctr)) + eval h0 a len_a * eval h0 b (len_a - ctr) );
+    swap_mul (getValue h0 b (len_a - ctr)) (pow2 (bitweight t (len_a - ctr)));
+    cut (True /\ eval h1 c (getLength h1 c) = eval h0 a len_a * pow2 (bitweight t (len_a - ctr)) * getValue h0 b (len_a - ctr) + eval h0 a len_a * eval h0 b (len_a - ctr) ) ;
   (* Verified up to this point *)
-  distributivity_add_right (eval h0 a len_a) (pow2 (bitweight t (len_a - ctr)) * getValue h0 b (len_a - ctr)) (eval h0 b (len_a - ctr));
-  cut (True /\ eval h1 c (getLength h1 c) = eval h0 a len_a * (pow2 (bitweight t (len_a - ctr)) * getValue h0 b (len_a - ctr) + eval h0 b (len_a - ctr))) ;
+    distributivity_add_right (eval h0 a len_a) (pow2 (bitweight t (len_a - ctr)) * getValue h0 b (len_a - ctr)) (eval h0 b (len_a - ctr));
+    cut (True /\ eval h1 c (getLength h1 c) = eval h0 a len_a * (pow2 (bitweight t (len_a - ctr)) * getValue h0 b (len_a - ctr) + eval h0 b (len_a - ctr))) ;
   () 
- 
+  )
 
 (* Helper lemma, ensures clause is self explainatory *)
 val auxiliary_lemma_7: a:int -> b:int -> c:int -> Lemma (ensures (a-(b-c)=a-b+c))
@@ -880,66 +892,69 @@ let multiplication c a b =
   let tmp2 = Bigint63 tmp (Bigint63.t a) in
   let h1 = 
     erase (ST.get()) in
+  erase (
+    eval_null h1 c (getLength h1 c);
+    max_value_of_null_lemma h1 c;
+    auxiliary_lemma_8 ();
+    auxiliary_lemma_9 (getLength h1 a);
   
-  eval_null h1 c (getLength h1 c);
-  max_value_of_null_lemma h1 c;
-  auxiliary_lemma_8 ();
-  auxiliary_lemma_9 (getLength h1 a);
-  
-  cut (eval h1 c (getLength h1 c) = 0 /\ True);
-  cut (eval h1 a (getLength h1 a) * eval h1 b (getLength h1 a - (getLength h1 a)) = 0 /\ True);
-  cut (eval h1 c (getLength h1 c) = eval h1 a (getLength h1 a) * eval h1 b (getLength h1 a - (getLength h1 a)) /\ True);
-  cut (maxValue h1 c = 0 /\ True);
-  cut ((getLength h1 a - (getLength h1 a)) * (maxValue h1 a * maxValue h1 b) = 0 /\ True);
-  cut (maxValue h1 c <= (getLength h1 a - (getLength h1 a)) * (maxValue h1 a * maxValue h1 b) /\ True);
-  cut (inHeap h1 a /\ inHeap h1 b /\ inHeap h1 c /\ inHeap h1 tmp2);
-  cut (getLength h1 a = getLength h1 b /\ getLength h1 tmp2 = getLength h1 a);
-  cut (getLength h1 a > 0 /\ getLength h1 c = 2 * getLength h1 a - 1);
+    cut (eval h1 c (getLength h1 c) = 0 /\ True);
+    cut (eval h1 a (getLength h1 a) * eval h1 b (getLength h1 a - (getLength h1 a)) = 0 /\ True);
+    cut (eval h1 c (getLength h1 c) = eval h1 a (getLength h1 a) * eval h1 b (getLength h1 a - (getLength h1 a)) /\ True);
+    cut (maxValue h1 c = 0 /\ True);
+    cut ((getLength h1 a - (getLength h1 a)) * (maxValue h1 a * maxValue h1 b) = 0 /\ True);
+    cut (maxValue h1 c <= (getLength h1 a - (getLength h1 a)) * (maxValue h1 a * maxValue h1 b) /\ True);
+    cut (inHeap h1 a /\ inHeap h1 b /\ inHeap h1 c /\ inHeap h1 tmp2);
+    cut (getLength h1 a = getLength h1 b /\ getLength h1 tmp2 = getLength h1 a);
+    cut (getLength h1 a > 0 /\ getLength h1 c = 2 * getLength h1 a - 1)
+  );
   let len = get_length a in
-  cut (getLength h1 a = len /\ True);
-  cut ( (Bigint63.t a = Bigint63.t b) 
-	/\ (Bigint63.t a = Bigint63.t c) 
-	/\ (Bigint63.t tmp2 = Bigint63.t a)
-	/\ (Bigint63.data c <> Bigint63.data a)	
-	/\ (Bigint63.data b <> Bigint63.data c)
-	/\ (Bigint63.data tmp2 <> Bigint63.data a) 
-	/\ (Bigint63.data tmp2 <> Bigint63.data b) 
-	/\ (Bigint63.data tmp2 <> Bigint63.data c) );
-  cut ( log (getLength h1 a) <= wordSize a - 2 /\ True);
-  cut ( maxSize h1 a <= (wordSize a - log (getLength h1 a) - 2) / 2
-			/\ maxSize h1 b <= (wordSize b - log (getLength h1 a) - 2) / 2);
-  cut (len <= getLength h1 a /\ True);
-  cut (maxSize h1 c <= wordSize a - 2 /\ True);
-  cut (maxValue h1 c <= (getLength h1 a - len) * (maxValue h1 a * maxValue h1 b) /\ True);
-  cut (eval h1 c (getLength h1 c) = eval h1 a (getLength h1 a) * eval h1 b (getLength h1 a - len) /\ True);
+  erase (
+    cut (getLength h1 a = len /\ True);
+    cut ( (Bigint63.t a = Bigint63.t b) 
+	  /\ (Bigint63.t a = Bigint63.t c) 
+	  /\ (Bigint63.t tmp2 = Bigint63.t a)
+	  /\ (Bigint63.data c <> Bigint63.data a)	
+	  /\ (Bigint63.data b <> Bigint63.data c)
+	  /\ (Bigint63.data tmp2 <> Bigint63.data a) 
+	  /\ (Bigint63.data tmp2 <> Bigint63.data b) 
+	  /\ (Bigint63.data tmp2 <> Bigint63.data c) );
+    cut ( log (getLength h1 a) <= wordSize a - 2 /\ True);
+    cut ( maxSize h1 a <= (wordSize a - log (getLength h1 a) - 2) / 2
+	  /\ maxSize h1 b <= (wordSize b - log (getLength h1 a) - 2) / 2);
+    cut (len <= getLength h1 a /\ True);
+    cut (maxSize h1 c <= wordSize a - 2 /\ True);
+    cut (maxValue h1 c <= (getLength h1 a - len) * (maxValue h1 a * maxValue h1 b) /\ True);
+    cut (eval h1 c (getLength h1 c) = eval h1 a (getLength h1 a) * eval h1 b (getLength h1 a - len) /\ True)
+  );
   
   multiplication_aux a b len c tmp2;
   let h2 = 
     erase (ST.get() ) in
   //cut (modifies !{Bigint63.data c} h0 h2);
-  
-  cut ((inHeap h0 a) /\ (inHeap h2 a)
-	       /\ (inHeap h0 b) /\ (inHeap h2 b)
-	       /\ (inHeap h0 c) /\ (inHeap h2 c) );
-  cut (getLength h0 a = getLength h0 b    /\ (getLength h0 a > 0) /\ (getLength h2 c = 2 * getLength h0 a - 1));
-  cut (IsNull h0 c  /\ (Bigint63.t a = Bigint63.t b)
-	       /\ (Bigint63.t a = Bigint63.t c)
-	       /\ (Bigint63.data c <> Bigint63.data a)
-	       /\ (Bigint63.data b <> Bigint63.data c) );
-
-  cut ( (wordSize a  - 2 >= log (getLength h0 a))
-	       /\ (maxSize h0 a <= (wordSize a - log (getLength h0 a) - 2) / 2)
-	       /\ (maxSize h0 b <= (wordSize b - log (getLength h0 a) - 2) / 2)
-	       /\ (maxSize h0 c <= wordSize a - 2)
-	       /\ (maxSize h2 c <= wordSize a - 2) );
-
-  eval_eq_lemma h0 h1 a a (getLength h0 a);
-  eval_eq_lemma h0 h1 b b (getLength h0 b);
-  
-  cut ( eval h2 c (getLength h2 c) = eval h0 a (getLength h0 a) * eval h0 b (getLength h0 b) /\ True);
-
-  cut ( modifies !{Bigint63.data c} h0 h2 );
-  //return_to_pool (Bigint63.data tmp2);
-  ()
-
+  erase (
+    cut ((inHeap h0 a) /\ (inHeap h2 a)
+	 /\ (inHeap h0 b) /\ (inHeap h2 b)
+	 /\ (inHeap h0 c) /\ (inHeap h2 c) );
+    cut (getLength h0 a = getLength h0 b    /\ (getLength h0 a > 0) /\ (getLength h2 c = 2 * getLength h0 a - 1));
+    cut (IsNull h0 c  /\ (Bigint63.t a = Bigint63.t b)
+	 /\ (Bigint63.t a = Bigint63.t c)
+	 /\ (Bigint63.data c <> Bigint63.data a)
+	 /\ (Bigint63.data b <> Bigint63.data c) );
+    
+    cut ( (wordSize a  - 2 >= log (getLength h0 a))
+	  /\ (maxSize h0 a <= (wordSize a - log (getLength h0 a) - 2) / 2)
+	  /\ (maxSize h0 b <= (wordSize b - log (getLength h0 a) - 2) / 2)
+	  /\ (maxSize h0 c <= wordSize a - 2)
+	  /\ (maxSize h2 c <= wordSize a - 2) );
+    
+    eval_eq_lemma h0 h1 a a (getLength h0 a);
+    eval_eq_lemma h0 h1 b b (getLength h0 b);
+    
+    cut ( eval h2 c (getLength h2 c) = eval h0 a (getLength h0 a) * eval h0 b (getLength h0 b) /\ True);
+    
+    cut ( modifies !{Bigint63.data c} h0 h2 );
+    //return_to_pool (Bigint63.data tmp2);
+    ()
+  )
 
